compiler/wasm/wbf_prelimScript.sml
@@ -1,5 +1,5 @@
 (*
-  Ancillaries for En- & De- coding between CWasm 1.ε AST & Wasm's binary format
+  Preliminaries for En- & De- coding between CWasm 1.ε AST & Wasm binary format
   such as:
   - Types
   - General (leb128) en-/de- coders
@@ -7,8 +7,20 @@
 *)
 Theory      wbf_prelim
 Ancestors   wasmLang leb128
-Libs        preamble wordsLib
+Libs        preamble wordsLib blastLib
 
+val ssaa = fn xs => [GSYM APPEND_ASSOC, Excl "APPEND_ASSOC"] @ xs
+val ssa  =          [GSYM APPEND_ASSOC, Excl "APPEND_ASSOC"]
+
+
+(*  Encoders ("enc_X") have type “:α -> word8 app_list option”
+    going from AST (elements) to optional (CakeML) app_lists of bytes
+      Though many encoders do not have a failure mode (they always return "SOME"),
+      for consistency, we have all encoders return options
+
+    Decoders ("dec_X") have type “”
+    take a stream of bytes and produce elements of the CWasm
+    AST (or an error) & additionally return the remaining bytes (stream)   *)
 
 (******************************)
 (*                            *)
@@ -16,19 +28,12 @@ Libs        preamble wordsLib
 (*                            *)
 (******************************)
 
-(*  Note:
-    Encoders ("enc_X") go from AST (elements) to optional (CakeML) app_lists of bytes
-      Though many encoders do not have a failure mode (always "SOME"), for consistency,
-      we have all encoders return options
-
-    Decoders ("dec_X") take a stream of bytes and produce elements of the CWasm
-    AST (or an error) & additionally return the remaining bytes (stream)     *)
-
 Type byte[pp]     = “:word8”
 Type byteSeq[pp]  = “:word8 list”
 Type byteCode[pp] = “:word8 app_list option”
 Type dcdr[pp]     = “:(mlstring + α) # byteSeq”
-(*  *)
+
+(* Some helpers for the dcdr monad *)
 Overload ret   = “λ bs a. (INR a, bs)”
 Overload err   = “(INL $ strlit "", [])”
 Overload error = “λ bs str. (INL $ strlit str,bs)”
@@ -46,36 +51,26 @@ val _ = set_fixity "[≤]" (Infixl 500);
 Overload "[≤]" =  “(λxs ys. LENGTH xs ≤ LENGTH ys): α list -> α list -> bool”
 
 val _ = set_fixity "+++" (Infixr 490);
-Overload "+++" = “Append”               (* cf cakeml/misc/miscScript.sml *)
+Overload "+++" = “Append”                       (* cf cakeml/misc/miscScript.sml *)
+
+val _ = set_fixity "a++" (Infixr 490);
+Overload "a++" = “λxs ys. append xs ++ ys”      (* cf cakeml/misc/miscScript.sml *)
 
 val _ = set_fixity ":::" (Infixr 485);
-Overload ":::" =  “(λx ys. Append (List [x:byte]) ys): byte -> byte app_list -> byte app_list”
+Overload ":::" =  “λx ys. Append (List [x:byte]) ys”
+
+Overload Soli[local] = “(SOME ∘ List): byteSeq -> byteCode”
 
 
 
 val _ = monadsyntax.enable_monadsyntax()
 val _ = monadsyntax.enable_monad "option"
 
-(******************************************)
-(*                                        *)
-(*     LEB128 Overloads and typecasts     *)
-(*                                        *)
-(******************************************)
-
-(**************************************************)
-(*   Functions, or rather, typecastings thereof   *)
-(**************************************************)
-
-(* Overload dec_u8  = “dec_unsigned_word : byteSeq -> (byte   # byteSeq) option”
-Overload dec_u32 = “dec_unsigned_word : byteSeq -> (word32 # byteSeq) option”
-Overload dec_u64 = “dec_unsigned_word : byteSeq -> (word64 # byteSeq) option”
-
-Overload dec_s8  = “dec_signed_word   : byteSeq -> (byte   # byteSeq) option”
-
-
-Overload enc_u64 = “enc_unsigned_word : word64 -> byteSeq”
-
-Overload enc_s8  = “enc_signed_word8  : byte   -> byteSeq” *)
+(******************************)
+(*                            *)
+(*     LEB128 "typecasts"     *)
+(*                            *)
+(******************************)
 
 Definition enc_s32_def:
   enc_s32 (w:word32) = SOME $ List $ enc_signed_word32 w
@@ -84,15 +79,6 @@ End
 Definition dec_s32_def:
   dec_s32 bs : word32 dcdr = lift $ dec_signed_word bs
 End
-
-Theorem dec_s32_shortens:
-  ∀bs rs _x. dec_s32 bs = (INR _x, rs) ⇒ rs [<] bs
-Proof
-     rpt gen_tac
-  \\ rw[dec_s32_def, AllCaseEqs()]
-  \\ dxrule dec_signed_word_shortens
-  \\ rewrite_tac[]
-QED
 
 
 Definition enc_s64_def:
@@ -103,106 +89,10 @@ Definition dec_s64_def:
   dec_s64 bs : word64 dcdr = lift $ dec_signed_word bs
 End
 
-Theorem dec_s64_shortens:
-  ∀bs rs _x. dec_s64 bs = (INR _x, rs) ⇒ rs [<] bs
-Proof
-     rpt gen_tac
-  \\ rw[dec_s64_def, AllCaseEqs()]
-  \\ dxrule dec_signed_word_shortens
-  \\ rewrite_tac[]
-QED
 
-
-
-Definition enc_u8_def:
-  enc_u8 (w:byte) = SOME $ List $ enc_unsigned_word w
-End
-
-Definition dec_u8_def:
-  dec_u8 bs : byte dcdr = lift $ dec_unsigned_word bs
-End
-
-Theorem dec_u8_shortens:
-  ∀bs rs _x. dec_u8 bs = (INR _x, rs) ⇒ rs [<] bs
-Proof
-     rpt gen_tac
-  \\ rw[dec_u8_def, AllCaseEqs()]
-  \\ dxrule dec_unsigned_word_shortens
-  \\ rewrite_tac[]
-QED
-
-
-Definition enc_u32_def:
-  enc_u32 (w:word32) = SOME $ List $ enc_unsigned_word w
-End
-
-Definition dec_u32_def:
-  dec_u32 bs : word32 dcdr = lift $ dec_unsigned_word bs
-End
-
-Theorem dec_u32_shortens:
-  ∀bs rs _x. dec_u32 bs = (INR _x, rs) ⇒ rs [<] bs
-Proof
-     rpt gen_tac
-  \\ rw[dec_u32_def, AllCaseEqs()]
-  \\ dxrule dec_unsigned_word_shortens
-  \\ rewrite_tac[]
-QED
-
-
-Definition enc_2u32_def:
-  enc_2u32 w v : byteCode = do
-    a <- enc_u32 w;
-    b <- enc_u32 v;
-    SOME $ a +++ b od
-End
-
-Definition dec_2u32_def:
-  dec_2u32 bs : (word32 # word32) dcdr =
-    case dec_u32 bs of (INL _, _) => err | (INR n, bs) =>
-    case dec_u32 bs of (INL _, _) => err | (INR m, bs) =>
-    ret bs (n,m)
-End
-
-Theorem dec_2u32_shortens:
-  ∀bs rs _x. dec_2u32 bs = (INR _x, rs) ⇒ rs [<] bs
-Proof
-     rpt gen_tac
-  \\ rw[dec_2u32_def, AllCaseEqs()]
-  \\ dxrule dec_u32_shortens
-  \\ dxrule dec_u32_shortens
-  \\ simp[]
-QED
-
-
-Definition enc_2u32_u8_def:
-  enc_2u32_u8 ofs al lid = do
-    a <- enc_2u32 ofs al;
-    b <- enc_u8 lid;
-    SOME $ a +++ b od
-End
-
-Definition dec_2u32_u8_def:
-  dec_2u32_u8 bs : (word32 # word32 # byte) dcdr =
-    case dec_2u32 bs of (INL _, _) => err | (INR (i,j), bs) =>
-    case dec_u8   bs of (INL _, _) => err | (INR k    , bs) =>
-    ret bs (i,j,k)
-End
-
-Theorem dec_2u32_u8_shortens:
-  ∀bs rs _x. dec_2u32_u8 bs = (INR _x, rs) ⇒ rs [<] bs
-Proof
-     rpt gen_tac
-  \\ rw[dec_2u32_u8_def, AllCaseEqs()]
-  \\ dxrule dec_2u32_shortens
-  \\ dxrule dec_u8_shortens
-  \\ simp[]
-QED
-
-
-(* Due to a perculiarity of Wasm (cf Block types - Index case from Wasm 2.0) *)
+(* we need s33 due to a perculiarity of Wasm (cf Block types - Index case from Wasm 2.0) *)
 Definition enc_s33_def:
-  enc_s33 (w:33 word) = SOME $
+  enc_s33 (w:33 word) = SOME $ List $
     if sw2sw ((w2w w):7 word) = w then
       enc_w7s [w2w w]
     else if sw2sw ((w2w w):14 word) = w then
@@ -229,10 +119,88 @@ Definition enc_s33_def:
                  w2w (w >>> 28)]
 End
 
-(* Overload dec_s33 = “dec_signed_word : byteSeq -> (33 word # byteSeq) option” *)
 Definition dec_s33_def:
   dec_s33 bs : (33 word) dcdr = lift $ dec_signed_word bs
 End
+
+
+
+
+
+Definition enc_u8_def:
+  enc_u8 (w:byte) = SOME $ List $ enc_unsigned_word w
+End
+
+Definition dec_u8_def:
+  dec_u8 bs : byte dcdr = lift $ dec_unsigned_word bs
+End
+
+
+Definition enc_u32_def:
+  enc_u32 (w:word32) = SOME $ List $ enc_unsigned_word w
+End
+
+Definition dec_u32_def:
+  dec_u32 bs : word32 dcdr = lift $ dec_unsigned_word bs
+End
+
+
+Definition enc_2u32_def:
+  enc_2u32 w v : byteCode = do
+    a <- enc_u32 w;
+    b <- enc_u32 v;
+    SOME $ a +++ b od
+End
+
+Definition dec_2u32_def:
+  dec_2u32 bs : (word32 # word32) dcdr =
+    case dec_u32 bs of (INL _, _) => err | (INR n, bs) =>
+    case dec_u32 bs of (INL _, _) => err | (INR m, bs) =>
+    ret bs (n,m)
+End
+
+
+Definition enc_2u32_u8_def:
+  enc_2u32_u8 ofs al lid = do
+    a <- enc_2u32 ofs al;
+    b <- enc_u8 lid;
+    SOME $ a +++ b od
+End
+
+Definition dec_2u32_u8_def:
+  dec_2u32_u8 bs : (word32 # word32 # byte) dcdr =
+    case dec_2u32 bs of (INL _, _) => err | (INR (i,j), bs) =>
+    case dec_u8   bs of (INL _, _) => err | (INR k    , bs) =>
+    ret bs (i,j,k)
+End
+
+
+
+
+
+(**************************************)
+(*                                    *)
+(*     LEB128 shortening theorems     *)
+(*                                    *)
+(**************************************)
+
+Theorem dec_s32_shortens:
+  ∀bs rs _x. dec_s32 bs = (INR _x, rs) ⇒ rs [<] bs
+Proof
+     rpt gen_tac
+  \\ rw[dec_s32_def, AllCaseEqs()]
+  \\ dxrule dec_signed_word_shortens
+  \\ rewrite_tac[]
+QED
+
+Theorem dec_s64_shortens:
+  ∀bs rs _x. dec_s64 bs = (INR _x, rs) ⇒ rs [<] bs
+Proof
+     rpt gen_tac
+  \\ rw[dec_s64_def, AllCaseEqs()]
+  \\ dxrule dec_signed_word_shortens
+  \\ rewrite_tac[]
+QED
 
 Theorem dec_s33_shortens:
   ∀bs rs _x. dec_s33 bs = (INR _x, rs) ⇒ rs [<] bs
@@ -243,3 +211,134 @@ Proof
   \\ rewrite_tac[]
 QED
 
+
+
+Theorem dec_u8_shortens:
+  ∀bs rs _x. dec_u8 bs = (INR _x, rs) ⇒ rs [<] bs
+Proof
+     rpt gen_tac
+  \\ rw[dec_u8_def, AllCaseEqs()]
+  \\ dxrule dec_unsigned_word_shortens
+  \\ rewrite_tac[]
+QED
+
+Theorem dec_u32_shortens:
+  ∀bs rs _x. dec_u32 bs = (INR _x, rs) ⇒ rs [<] bs
+Proof
+     rpt gen_tac
+  \\ rw[dec_u32_def, AllCaseEqs()]
+  \\ dxrule dec_unsigned_word_shortens
+  \\ rewrite_tac[]
+QED
+
+Theorem dec_2u32_shortens:
+  ∀bs rs _x. dec_2u32 bs = (INR _x, rs) ⇒ rs [<] bs
+Proof
+     rpt gen_tac
+  \\ rw[dec_2u32_def, AllCaseEqs()]
+  \\ dxrule dec_u32_shortens
+  \\ dxrule dec_u32_shortens
+  \\ simp[]
+QED
+
+Theorem dec_2u32_u8_shortens:
+  ∀bs rs _x. dec_2u32_u8 bs = (INR _x, rs) ⇒ rs [<] bs
+Proof
+     rpt gen_tac
+  \\ rw[dec_2u32_u8_def, AllCaseEqs()]
+  \\ dxrule dec_2u32_shortens
+  \\ dxrule dec_u8_shortens
+  \\ simp[]
+QED
+
+
+
+
+
+(***********************************)
+(*                                 *)
+(*     LEB128 dec-enc theorems     *)
+(*                                 *)
+(***********************************)
+
+Theorem dec_enc_s32:
+  ∀x encx. enc_s32 x = SOME encx ⇒
+  ∀rest. dec_s32 $ append encx ++ rest = (INR x, rest)
+Proof
+     rw[enc_s32_def, dec_s32_def, AllCaseEqs()]
+  \\ rw[append_def, dec_enc_signed_word32]
+QED
+
+Theorem dec_enc_s64:
+  ∀x encx. enc_s64 x = SOME encx ⇒
+  ∀rest. dec_s64 $ append encx ++ rest = (INR x, rest)
+Proof
+     rw[enc_s64_def, dec_s64_def, AllCaseEqs()]
+  \\ rw[append_def, dec_enc_signed_word64]
+QED
+
+Theorem dec_enc_s33:
+  ∀x encx. enc_s33 x = SOME encx ⇒
+  ∀rest. dec_s33 $ append encx ++ rest = (INR x, rest)
+Proof
+     rw[dec_s33_def, AllCaseEqs(), enc_s33_def]
+  >> rw[append_def, dec_signed_word_def, dec_enc_w7s, or_w7s_def]
+  >> pop_assum mp_tac
+  >> first_x_assum mp_tac
+  >> BBLAST_TAC
+QED
+
+Theorem dec_enc_u8:
+  ∀x encx. enc_u8 x = SOME encx ⇒
+  ∀rest. dec_u8 $ append encx ++ rest = (INR x, rest)
+Proof
+     rw[dec_u8_def, enc_u8_def, AllCaseEqs()]
+  \\ rw[append_def, dec_enc_unsigned_word]
+QED
+
+Theorem dec_enc_u32:
+  ∀x encx. enc_u32 x = SOME encx ⇒
+  ∀rest. dec_u32 $ append encx ++ rest = (INR x, rest)
+Proof
+     rw[dec_u32_def, enc_u32_def, AllCaseEqs()]
+  \\ rw[append_def, dec_enc_unsigned_word]
+QED
+
+Theorem dec_enc_2u32:
+  ∀x y encx. enc_2u32 x y = SOME encx ⇒
+  ∀rest. dec_2u32 $ append encx ++ rest = (INR (x,y), rest)
+Proof
+     rw[dec_2u32_def, enc_2u32_def, AllCaseEqs()]
+  \\ simp $ ssa
+  \\ imp_res_tac dec_enc_u32
+  \\ asm_rewrite_tac[]
+  \\ gvs[]
+QED
+
+Theorem dec_enc_2u32_u8:
+  ∀x y z encx. enc_2u32_u8 x y z = SOME encx ⇒
+  ∀rest. dec_2u32_u8 $ append encx ++ rest = (INR (x,y,z), rest)
+Proof
+     rw[dec_2u32_u8_def, enc_2u32_u8_def, AllCaseEqs()]
+  \\ simp $ ssa
+  \\ imp_res_tac dec_enc_2u32
+  \\ asm_rewrite_tac[]
+  \\ gvs[]
+  \\ imp_res_tac dec_enc_u8
+  \\ gvs[]
+QED
+
+
+
+
+
+(* Overload dec_u8  = “dec_unsigned_word : byteSeq -> (byte   # byteSeq) option”
+Overload dec_u32 = “dec_unsigned_word : byteSeq -> (word32 # byteSeq) option”
+Overload dec_u64 = “dec_unsigned_word : byteSeq -> (word64 # byteSeq) option”
+
+Overload dec_s8  = “dec_signed_word   : byteSeq -> (byte   # byteSeq) option”
+
+
+Overload enc_u64 = “enc_unsigned_word : word64 -> byteSeq”
+
+Overload enc_s8  = “enc_signed_word8  : byte   -> byteSeq” *)
