compiler/wasm/wbf_thmsScript.sml
@@ -15,43 +15,43 @@ val ssa  =          [GSYM APPEND_ASSOC, Excl "APPEND_ASSOC"]
 (***************************)
 
 Theorem enc_numI_nEmp_nTermB:
-  ∀i encbs. enc_numI i = SOME encbs ⇒
-  ∃b bs. append encbs =  b::bs ∧ b ≠ endB ∧ b ≠ elseB
+  ∀x encx. enc_numI x = SOME encx ⇒
+  ∃b bs. append encx =  b::bs ∧ b ≠ endB ∧ b ≠ elseB
 Proof
   rw[Once enc_numI_def, AllCaseEqs()] >> simp[]
 QED
 
 Theorem enc_paraI_nEmp_nTermB:
-  ∀i. enc_paraI i = SOME encbs ⇒
-  ∃b bs. append encbs =  b::bs ∧ b ≠ endB ∧ b ≠ elseB
+  ∀x encx. enc_paraI x = SOME encx ⇒
+  ∃b bs. append encx =  b::bs ∧ b ≠ endB ∧ b ≠ elseB
 Proof
   Cases \\ simp[Once enc_paraI_def, AllCaseEqs()]
 QED
 
 Theorem enc_varI_nEmp_nTermB:
-  ∀i. enc_varI i = SOME encbs ⇒
-  ∃b bs. append encbs = b::bs ∧ b ≠ endB ∧ b ≠ elseB
+  ∀x encx. enc_varI x = SOME encx ⇒
+  ∃b bs. append encx = b::bs ∧ b ≠ endB ∧ b ≠ elseB
 Proof
   rw[Once enc_varI_def, AllCaseEqs()] >> simp[]
 QED
 
 Theorem enc_loadI_nEmp_nTermB:
-  ∀i. enc_loadI i = SOME encbs ⇒
-  ∃b bs. append encbs = b::bs ∧ b ≠ endB ∧ b ≠ elseB
+  ∀x encx. enc_loadI x = SOME encx ⇒
+  ∃b bs. append encx = b::bs ∧ b ≠ endB ∧ b ≠ elseB
 Proof
   rw[Once enc_loadI_def, AllCaseEqs()] >> simp[]
 QED
 
 Theorem enc_storeI_nEmp_nTermB:
-  ∀i. enc_storeI i = SOME encbs ⇒
-  ∃b bs. append encbs = b::bs ∧ b ≠ endB ∧ b ≠ elseB
+  ∀x encx. enc_storeI x = SOME encx ⇒
+  ∃b bs. append encx = b::bs ∧ b ≠ endB ∧ b ≠ elseB
 Proof
   rw[Once enc_storeI_def, AllCaseEqs()] >> simp[]
 QED
 
 Theorem enc_instr_nEmp_nTermB:
-  ∀i enci. enc_instr i = SOME enci ⇒
-  ∃b bs. append enci = b::bs ∧ b ≠ endB ∧ b ≠ elseB
+  ∀x encx. enc_instr x = SOME encx ⇒
+  ∃b bs. append encx = b::bs ∧ b ≠ endB ∧ b ≠ elseB
 Proof
   Cases
   >> rw[Once enc_instr_def, AllCaseEqs()]
@@ -64,8 +64,8 @@ Proof
 QED
 
 Theorem num_cf_instr_disjoint:
-  ∀i enci. enc_numI i = SOME enci ⇒
-  ∃b bs. append enci = b::bs ⇒
+  ∀x encx. enc_numI x = SOME encx ⇒
+  ∃b bs. append encx = b::bs ⇒
   b ≠ unrOC ∧ b ≠ nopOC ∧ b ≠ blkOC ∧
   b ≠ lopOC ∧ b ≠ if_OC ∧ b ≠ br_OC ∧
   b ≠ briOC ∧ b ≠ brtOC ∧ b ≠ retOC ∧
@@ -77,8 +77,8 @@ Proof
 QED
 
 Theorem para_cf_instr_disjoint:
-  ∀i enci. enc_paraI i = SOME enci ⇒
-  ∃b bs. append enci = b::bs ⇒
+  ∀x encx. enc_paraI x = SOME encx ⇒
+  ∃b bs. append encx = b::bs ⇒
   b ≠ unrOC ∧ b ≠ nopOC ∧ b ≠ blkOC ∧
   b ≠ lopOC ∧ b ≠ if_OC ∧ b ≠ br_OC ∧
   b ≠ briOC ∧ b ≠ brtOC ∧ b ≠ retOC ∧
@@ -89,8 +89,8 @@ Proof
 QED
 
 Theorem var_cf_instr_disjoint:
-  ∀i enci. enc_varI i = SOME enci ⇒
-  ∃b bs. append enci =  b::bs ⇒
+  ∀x encx. enc_varI x = SOME encx ⇒
+  ∃b bs. append encx =  b::bs ⇒
   b ≠ unrOC ∧ b ≠ nopOC ∧ b ≠ blkOC ∧
   b ≠ lopOC ∧ b ≠ if_OC ∧ b ≠ br_OC ∧
   b ≠ briOC ∧ b ≠ brtOC ∧ b ≠ retOC ∧
@@ -102,8 +102,8 @@ Proof
 QED
 
 Theorem load_cf_instr_disjoint:
-  ∀i enci. enc_loadI i = SOME enci ⇒
-  ∃b bs. append enci =  b::bs ⇒
+  ∀x encx. enc_loadI x = SOME encx ⇒
+  ∃b bs. append encx =  b::bs ⇒
   b ≠ unrOC ∧ b ≠ nopOC ∧ b ≠ blkOC ∧
   b ≠ lopOC ∧ b ≠ if_OC ∧ b ≠ br_OC ∧
   b ≠ briOC ∧ b ≠ brtOC ∧ b ≠ retOC ∧
@@ -115,8 +115,8 @@ Proof
 QED
 
 Theorem store_cf_instr_disjoint:
-  ∀i enci. enc_storeI i = SOME enci ⇒
-  ∃b bs. append enci = b::bs ⇒
+  ∀x encx. enc_storeI x = SOME encx ⇒
+  ∃b bs. append encx = b::bs ⇒
   b ≠ unrOC ∧ b ≠ nopOC ∧ b ≠ blkOC ∧
   b ≠ lopOC ∧ b ≠ if_OC ∧ b ≠ br_OC ∧
   b ≠ briOC ∧ b ≠ brtOC ∧ b ≠ retOC ∧
@@ -128,15 +128,15 @@ Proof
 QED
 
 Theorem var_para_disjoint:
-  ∀p encp. enc_paraI p = SOME encp ⇒
-  ∀rest. ∃ e. dec_varI (append encp ++ rest) = (INL e, append encp ++ rest)
+  ∀x encx. enc_paraI x = SOME encx ⇒
+  ∀rest. ∃e. dec_varI (append encx ++ rest) = (INL e, append encx ++ rest)
 Proof
   Cases >> simp[enc_paraI_def, dec_varI_def]
 QED
 
 Theorem var_num_disjoint:
-  ∀n encn. enc_numI n = SOME encn ⇒
-  ∀rest. ∃ e. dec_varI (append encn ++ rest) = (INL e, append encn ++ rest)
+  ∀x encx. enc_numI x = SOME encx ⇒
+  ∀rest. ∃e. dec_varI (append encx ++ rest) = (INL e, append encx ++ rest)
 Proof
   Cases >> gen_tac
   >> rw[enc_numI_def, AllCaseEqs()]
@@ -144,8 +144,8 @@ Proof
 QED
 
 Theorem para_num_disjoint:
-  ∀i enci. enc_numI i = SOME enci ⇒
-  ∀rest. ∃ e. dec_paraI (append enci ++ rest) = (INL e, append enci ++ rest)
+  ∀x encx. enc_numI x = SOME encx ⇒
+  ∀rest. ∃e. dec_paraI (append encx ++ rest) = (INL e, append encx ++ rest)
 Proof
   Cases >> gen_tac
   >> rw[enc_numI_def, AllCaseEqs()]
@@ -153,8 +153,8 @@ Proof
 QED
 
 Theorem var_load_disjoint:
-  ∀i enci. enc_loadI i = SOME enci ⇒
-  ∀rest. ∃ e. dec_varI (append enci ++ rest) = (INL e, append enci ++ rest)
+  ∀x encx. enc_loadI x = SOME encx ⇒
+  ∀rest. ∃e. dec_varI (append encx ++ rest) = (INL e, append encx ++ rest)
 Proof
   Cases >> gen_tac
   >> simp[enc_loadI_def, AllCaseEqs()]
@@ -163,8 +163,8 @@ Proof
 QED
 
 Theorem para_load_disjoint:
-  ∀i enci. enc_loadI i = SOME enci ⇒
-  ∀l rest. ∃ e. dec_paraI (append enci ++ rest) = (INL e, append enci ++ rest)
+  ∀x encx. enc_loadI x = SOME encx ⇒
+  ∀rest. ∃e. dec_paraI (append encx ++ rest) = (INL e, append encx ++ rest)
 Proof
   Cases >> gen_tac
   >> simp[enc_loadI_def, AllCaseEqs()]
@@ -173,8 +173,8 @@ Proof
 QED
 
 Theorem num_load_disjoint:
-  ∀i enci. enc_loadI i = SOME enci ⇒
-  ∀l rest. ∃ e. dec_numI (append enci ++ rest) = (INL e, append enci ++ rest)
+  ∀x encx. enc_loadI x = SOME encx ⇒
+  ∀rest. ∃e. dec_numI (append encx ++ rest) = (INL e, append encx ++ rest)
 Proof
   Cases >> gen_tac
   >> simp[enc_loadI_def, AllCaseEqs()]
@@ -183,8 +183,8 @@ Proof
 QED
 
 Theorem var_store_disjoint:
-  ∀i enci. enc_storeI i = SOME enci ⇒
-  ∀l rest. ∃ e. dec_varI (append enci ++ rest) = (INL e, append enci ++ rest)
+  ∀x encx. enc_storeI x = SOME encx ⇒
+  ∀rest. ∃e. dec_varI (append encx ++ rest) = (INL e, append encx ++ rest)
 Proof
   Cases >> gen_tac
   >> simp[enc_storeI_def, AllCaseEqs()]
@@ -193,8 +193,8 @@ Proof
 QED
 
 Theorem para_store_disjoint:
-  ∀i enci. enc_storeI i = SOME enci ⇒
-  ∀l rest. ∃ e. dec_paraI (append enci ++ rest) = (INL e, append enci ++ rest)
+  ∀x encx. enc_storeI x = SOME encx ⇒
+  ∀rest. ∃e. dec_paraI (append encx ++ rest) = (INL e, append encx ++ rest)
 Proof
   Cases >> gen_tac
   >> simp[enc_storeI_def, AllCaseEqs()]
@@ -203,8 +203,8 @@ Proof
 QED
 
 Theorem num_store_disjoint:
-  ∀i enci. enc_storeI i = SOME enci ⇒
-  ∀l rest. ∃ e. dec_numI (append enci ++ rest) = (INL e, append enci ++ rest)
+  ∀x encx. enc_storeI x = SOME encx ⇒
+  ∀rest. ∃e. dec_numI (append encx ++ rest) = (INL e, append encx ++ rest)
 Proof
   Cases >> gen_tac
   >> simp[enc_storeI_def, AllCaseEqs()]
@@ -212,19 +212,22 @@ Proof
   >> gvs[dec_numI_def]
 QED
 
-(*
 Theorem load_store_disjoint:
-  ∀i enci. enc_storeI i = SOME enci ⇒
-  ∀l rest. ∃ e. dec_loadI (append enci ++ rest) = (INL e, append enci ++ rest)
+  ∀x encx. enc_storeI x = SOME encx ⇒
+  ∀rest. ∃e. dec_loadI (append encx ++ rest) = (INL e, append encx ++ rest)
 Proof
-  >> simp[enc_storeI_def, AllCaseEqs()]
-  >> rpt strip_tac
+  simp[enc_storeI_def, AllCaseEqs()]
+  >> rpt strip_tac >> imp_res_tac dec_enc_2u32
   >> gvs[dec_loadI_def]
-  Cases
-  rw[enc_storeI_def] >> Cases_on `i`
-  Cases >> gen_tac
 QED
 
+Theorem enc_valtype_nEmp_n0x40:
+  ∀x encx. enc_valtype x = SOME encx ⇒ ∃b bs. append encx = b::bs ∧ b ≠ 0x40w
+Proof
+  Cases
+  >> Cases_on `w`
+  >> rw[enc_valtype_def, AllCaseEqs(), bvtype_nchotomy]
+QED
 
 
 
@@ -238,73 +241,33 @@ QED
 (* MM's neat trick to check if we're making progress *)
 fun print_dot_tac h = (print "."; all_tac h);
 
-(**************)
-(*   leb128   *)
-(**************)
-
-Theorem dec_enc_u8:
-  ∀x encx. enc_u8 x = SOME encx ⇒
-  ∀rest. dec_u8 $ append encx ++ rest = (INR x, rest)
-Proof
-     rw[dec_u8_def, enc_u8_def, AllCaseEqs()]
-  \\ rw[append_def, dec_enc_unsigned_word]
-QED
-
-Theorem dec_enc_u32:
-  ∀x encx. enc_u32 x = SOME encx ⇒
-  ∀rest. dec_u32 $ append encx ++ rest = (INR x, rest)
-Proof
-     rw[dec_u32_def, enc_u32_def, AllCaseEqs()]
-  \\ rw[append_def, dec_enc_unsigned_word]
-QED
-
-Theorem dec_enc_2u32:
-  ∀x encx. enc_2u32 x y = SOME encx ⇒
-  ∀rest. dec_2u32 $ append encx ++ rest = (INR (x,y), rest)
-Proof
-     rw[dec_2u32_def, enc_2u32_def, AllCaseEqs()]
-  \\ simp $ ssa
-
-  \\ imp_res_tac dec_enc_u32
-  \\ asm_rewrite_tac[]
-  \\ strip_tac
-  \\
-  \\ dxrule dec_enc_u32
-[]
-  \\ rw[append_def, dec_enc_u32]
-  \\ rw[append_aux_def, dec_enc_u32]
-
-QED
-
-
-
-
-
 (*****************************************)
 (*   Vectors (not vector instructions)   *)
 (*****************************************)
 
 Theorem dec_enc_vector:
-  ∀dec enc is encis.
+  ∀enc dec is encis.
     enc_vector enc is = SOME encis ∧
     (∀x encx rs. enc x = SOME encx ⇒ dec (append encx ++ rs) = (INR x,rs))
     ⇒
-    ∀rest. dec_vector dec (append encis ++ rest) = (INR is, rest)
+    ∀rest. dec_vector dec (encis a++ rest) = (INR is, rest)
 Proof
-
   rpt strip_tac
   \\ last_x_assum mp_tac
-  \\ rw[dec_vector_def, enc_vector_def, AllCaseEqs()]
-  \\ gvs $ ssaa [GSYM NOT_LESS]
+  \\ simp[dec_vector_def, enc_vector_def, AllCaseEqs(), GSYM NOT_LESS]
+  \\ rpt strip_tac
+  \\ gvs ssa
+  \\ imp_res_tac dec_enc_u32
+  \\ simp[]
+  \\ (* tidy up from dec enc vec pf *)
+     ntac 2 $ pop_assum kall_tac
+  (* dec_enc_list *)
   \\ pop_assum mp_tac
   \\ qid_spec_tac ‘rest’
   \\ qid_spec_tac ‘encxs’
   \\ qid_spec_tac ‘is’
   \\ Induct
   >> simp[enc_list_def, Once dec_list_def, CaseEq "sum", CaseEq "prod"]
-
-cheat
-
   \\ rpt strip_tac
   \\ gvs[]
   \\ last_x_assum dxrule
@@ -312,65 +275,47 @@ cheat
 QED
 
 
-
-
-
 (*************)
 (*   Types   *)
 (*************)
 
-Theorem dec_enc_valtype[simp]:
-  ∀t rest. dec_valtype (enc_valtype t ++ rest) = (INR t, rest)
+Theorem dec_enc_valtype:
+  ∀x encx. enc_valtype x = SOME encx ⇒
+  ∀rest. dec_valtype (encx a++ rest) = (INR x, rest)
 Proof
-     rpt gen_tac
-  \\ ‘∃ val. enc_valtype t = val’ by simp []
-  \\ asm_rewrite_tac[]
-  \\ pop_assum mp_tac
-  \\ simp[enc_valtype_def, AllCaseEqs(), bvtype_nchotomy]
-  \\ rpt strip_tac
-    >> gvs[dec_valtype_def]
+     Cases
+  \\ simp[bvtype_nchotomy, enc_valtype_def, dec_valtype_def, AllCaseEqs()]
+  \\ Cases_on `w`
+  >> simp[]
 QED
 
 Theorem dec_enc_functype:
-  ∀sg encsg rest.
-    enc_functype sg = SOME encsg ⇒
-    dec_functype (encsg ++ rest) = (INR sg, rest)
+  ∀sg encsg. enc_functype sg = SOME encsg ⇒
+  ∀rest. dec_functype (encsg a++ rest) = (INR sg, rest)
 Proof
-     rw[AllCaseEqs(), enc_functype_def]
+     rw[enc_functype_def, AllCaseEqs()]
   \\ PairCases_on ‘sg’
   \\ gvs[dec_functype_def, AllCaseEqs()]
-  \\ dxrule dec_enc_vector
-  \\ disch_then $ qspec_then ‘dec_valtype’ assume_tac
-  \\ dxrule dec_enc_vector
-  \\ disch_then $ qspec_then ‘dec_valtype’ assume_tac
+  \\ rpt $ dxrule dec_enc_vector
+  \\ rpt $ disch_then $ qspec_then ‘dec_valtype’ assume_tac
   \\ gvs[dec_enc_valtype]
   \\ simp ssa
 QED
 
-Theorem dec_enc_limits[simp]:
-  ∀ lim rest. dec_limits (enc_limits lim ++ rest) = (INR lim, rest)
+Theorem dec_enc_limits:
+  ∀x encx. enc_limits x = SOME encx ⇒
+  ∀ rest. dec_limits (encx a++ rest) = (INR x, rest)
 Proof
-     rpt gen_tac
-  \\ ‘∃ val. enc_limits lim = val’ by simp []
-  \\ asm_rewrite_tac[]
-  \\ pop_assum mp_tac
-  \\ rewrite_tac[enc_limits_def]
-  \\ simp[AllCaseEqs()]
-  \\ rpt strip_tac
-    >> gvs[dec_limits_def]
+     rw[enc_limits_def, AllCaseEqs()]
+  >> simp[dec_limits_def, AllCaseEqs(), dec_enc_u32, dec_enc_2u32]
 QED
 
-Theorem dec_enc_globaltype[simp]:
-  ∀ x rest. dec_globaltype (enc_globaltype x ++ rest) = (INR x, rest)
+Theorem dec_enc_globaltype:
+  ∀x encx. enc_globaltype x = SOME encx ⇒
+  ∀rest. dec_globaltype (encx a++ rest) = (INR x, rest)
 Proof
-     rpt gen_tac
-  \\ ‘∃ val. enc_globaltype x = val’ by simp []
-  \\ asm_rewrite_tac[]
-  \\ pop_assum mp_tac
-  \\ rewrite_tac[enc_globaltype_def]
-  \\ simp[AllCaseEqs()]
-  \\ rpt strip_tac
-    >> gvs $ ssaa [dec_globaltype_def, dec_enc_valtype]
+     rw[enc_globaltype_def, dec_globaltype_def, AllCaseEqs()]
+  >> simp $ ssaa [dec_enc_valtype]
 QED
 
 
@@ -379,59 +324,47 @@ QED
 (*   Instructions (hierarchically lower)   *)
 (*******************************************)
 
-Theorem dec_enc_numI[simp]:
-  ∀ i rest. dec_numI (enc_numI i ++ rest) = (INR i, rest)
+Theorem dec_enc_numI:
+  ∀x encx. enc_numI x = SOME encx ⇒
+  ∀rest. dec_numI (encx a++ rest) = (INR x, rest)
 Proof
-     rpt gen_tac
-  \\ ‘∃res. enc_numI i = res’ by simp []
-  \\ asm_rewrite_tac []
-  \\ pop_assum mp_tac
-  \\ rewrite_tac [enc_numI_def]
-  \\ simp[AllCaseEqs(), bvtype_nchotomy, convert_op_nchotomy]
-  \\ rpt strip_tac
-  (* single byte encoding cases *)
-  >> asm_rewrite_tac[APPEND, dec_numI_def]
-  >> simp[AllCaseEqs()]
-    (* cases requiring further encoding (of their "immediates") *)
-    >> (
-      pop_assum sym_sub_tac
-      >- simp[dec_numI_def, AllCaseEqs()]
-    )
+     rw[enc_numI_def, AllCaseEqs(), bvtype_nchotomy, convert_op_nchotomy]
+  >>~- ([‘N_const32’], simp[dec_numI_def, AllCaseEqs(), dec_enc_s32])
+  >>~- ([‘N_const64’], simp[dec_numI_def, AllCaseEqs(), dec_enc_s64])
+  >> simp[dec_numI_def]
 QED
 
-Theorem dec_enc_paraI[simp]:
-  ∀ i rest. dec_paraI (enc_paraI i ++ rest) = (INR i, rest)
+Theorem dec_enc_paraI:
+  ∀x encx. enc_paraI x = SOME encx ⇒
+  ∀rest. dec_paraI (encx a++ rest) = (INR x, rest)
 Proof
-  rw[enc_paraI_def] \\ every_case_tac \\ rw[dec_paraI_def]
+  Cases
+  >> rw[enc_paraI_def, AllCaseEqs()]
+  >> simp[dec_paraI_def]
 QED
 
-Theorem dec_enc_varI[simp]:
-  ∀ i rest. dec_varI (enc_varI i ++ rest) = (INR i, rest)
+Theorem dec_enc_varI:
+  ∀x encx. enc_varI x = SOME encx ⇒
+  ∀rest. dec_varI (encx a++ rest) = (INR x, rest)
 Proof
-  rw[enc_varI_def] \\ every_case_tac \\ rw[dec_varI_def, dec_enc_unsigned_word]
+     rw[enc_varI_def, AllCaseEqs()]
+  >> simp[dec_varI_def, AllCaseEqs(), dec_enc_u32]
 QED
 
-Theorem dec_enc_loadI[simp]:
-  ∀ i rest. dec_loadI (enc_loadI i ++ rest) = (INR i, rest)
+Theorem dec_enc_loadI:
+  ∀x encx. enc_loadI x = SOME encx ⇒
+  ∀rest. dec_loadI (encx a++ rest) = (INR x, rest)
 Proof
-  rpt gen_tac
-  \\ ‘∃res. enc_loadI i = res’ by simp [] >> asm_rewrite_tac[]
-  \\ pop_assum mp_tac
-  \\ simp[enc_loadI_def, AllCaseEqs(), bvtype_nchotomy]
-  \\ rpt strip_tac
-    >> ( pop_assum sym_sub_tac >- simp[dec_loadI_def, AllCaseEqs()] )
+     rw[enc_loadI_def, AllCaseEqs(), bvtype_nchotomy]
+  >> simp[dec_loadI_def, AllCaseEqs(), dec_enc_2u32]
 QED
 
-Theorem dec_enc_storeI[simp]:
-  ∀ i rest. dec_storeI (enc_storeI i ++ rest) = (INR i, rest)
+Theorem dec_enc_storeI:
+  ∀x encx. enc_storeI x = SOME encx ⇒
+  ∀rest. dec_storeI (encx a++ rest) = (INR x, rest)
 Proof
-  rpt gen_tac
-  \\ ‘∃res. enc_storeI i = res’ by simp []
-  \\ asm_rewrite_tac []
-  \\ pop_assum mp_tac
-  \\ simp[enc_storeI_def, AllCaseEqs(), bvtype_nchotomy]
-  \\ rpt strip_tac
-    >> gvs[dec_storeI_def]
+     rw[enc_storeI_def, AllCaseEqs(), bvtype_nchotomy]
+  >> simp[dec_storeI_def, AllCaseEqs(), dec_enc_2u32]
 QED
 
 
@@ -442,35 +375,26 @@ QED
 (*                                            *)
 (**********************************************)
 
-Theorem dec_enc_blocktype[simp]:
-  ∀b rest. dec_blocktype (enc_blocktype b ++ rest) = (INR b, rest)
+Theorem dec_enc_blocktype:
+  ∀x encx. enc_blocktype x = SOME encx ⇒
+  ∀rest. dec_blocktype (encx a++ rest) = (INR x, rest)
 Proof
-  rpt strip_tac
-  \\ ‘∃ val. enc_blocktype b = val’ by simp []
-  \\ asm_rewrite_tac[]
-  \\ pop_assum mp_tac
-  \\ gvs[enc_blocktype_def, AllCaseEqs()]
-  \\ rpt strip_tac
-  >> gvs[dec_blocktype_def]
-  \\ Cases_on ‘vt’ \\ Cases_on ‘w’
-  >> simp[enc_valtype_def, AllCaseEqs()]
+  rw[enc_blocktype_def, AllCaseEqs()]
+  >> simp[dec_blocktype_def, AllCaseEqs()]
+  \\ imp_res_tac enc_valtype_nEmp_n0x40
+  \\ imp_res_tac dec_enc_valtype
+  \\ gvs[]
 QED
 
-
-Theorem dec_enc_lift_u32[simp]:
-  ∀b rest. lift_dec_u32 (enc_u32 b ++ rest) = (INR b, rest)
-Proof
-  rpt gen_tac
-  \\ simp[lift_dec_u32_def]
-QED
 
 Theorem dec_enc_indxs:
-  ∀bs encbs rest. enc_indxs bs = SOME encbs ⇒
-  dec_indxs (encbs ++ rest) = (INR bs, rest)
+  ∀x encx. enc_indxs x = SOME encx ⇒
+  ∀rest. dec_indxs (encx a++ rest) = (INR x, rest)
 Proof
   rpt strip_tac
-  \\ dxrule_at Any dec_enc_vector
-  \\ simp[dec_enc_lift_u32]
+  \\ qspec_then ‘enc_u32’ irule dec_enc_vector
+  \\ assume_tac dec_enc_u32
+  \\ simp[]
 QED
 
 
@@ -479,32 +403,78 @@ QED
 
 Overload exprB[local] = “λe. if e then endB else elseB”
 
+(*
 (* [Note] on "dc": Here the statements says that if we encode an expr (e=T), then we _must_ see an endB (¬e ∨ dc=F)
    But if we're encoding a then-arm (e=F), then we (dc:=)don't care whether the decoder gets a T or F flag *)
 Theorem dec_enc_instructions:
-  (∀e is dc encis rs. enc_instr_list e is = SOME encis ⇒ dec_instr_list (¬e ∨ dc) (encis ++ rs) = (INR (exprB e,is), rs)) ∧
-  (∀  i     enci  rs. enc_instr        i  = SOME enci  ⇒ dec_instr                (enci  ++ rs) = (INR          i  , rs))
+  (∀e xs dc encxs rs. enc_instr_list e xs = SOME encxs ⇒ dec_instr_list (¬e ∨ dc) (encxs a++ rs) = ret rs $ (exprB e,xs)) ∧
+  (∀  x     encx  rs. enc_instr        x  = SOME encx  ⇒ dec_instr                (encx  a++ rs) = ret rs $          x  )
 Proof
   (* askyk - how to: golf? make more ergonomic and/or robust? *)
   (* Note - all the work is really done in the instr (as opposed to instr_list) case *)
+
   ho_match_mp_tac enc_instr_ind
   \\ simp[]
   \\ rpt strip_tac
   >> pop_assum mp_tac
-  >-( Cases_on ‘e’ >> simp[enc_instr_def, Once dec_instr_def] )
   >-(
-    simp[Once enc_instr_def]
-    >> rpt strip_tac
-    >> imp_res_tac enc_instr_nEmp_nTermB
-    >> gvs[]
-    >> simp[Once dec_instr_def]
-    >> simp ssa
-    )
+     Cases_on ‘e’ >> simp[enc_instr_def, Once dec_instr_def]
+  )
+  >-(
+     simp[Once enc_instr_def]
+     >> rpt strip_tac
+     >> imp_res_tac enc_instr_nEmp_nTermB
+     >> gvs[]
+     >> simp[Once dec_instr_def]
+     >> simp ssa
+  )
+
   \\
-    Cases_on ‘i’
+    Cases_on ‘x’
     >> rw[Once enc_instr_def]
-    >> rewrite_tac[APPEND, dec_instr_def]
+    >> imp_res_tac dec_enc_u32
+    >> imp_res_tac dec_enc_indxs
+    >> imp_res_tac dec_enc_functype
+    >> imp_res_tac dec_enc_blocktype
     >> simp ssa
+    >> simp[dec_instr_def]
+    (**)
+
+>>~- ([‘enc_blocktype’],
+    simp ssa
+    >> pop_assum drule_all
+    >> imp_res_tac dec_enc_blocktype
+    >> strip_tac
+    >> simp[]
+)
+cheat
+
+imp_res_tac dec_enc_u32
+simp[]
+pop_assum mp_tac
+disch_then $ qspec_then `rs` assume_tac
+gvs[]
+asm_rewrite_tac[]
+simp[]
+simp[]
+simp[AllCaseEqs()]
+assume_tac dec_enc_u32
+simp[append_def]
+simp[append_aux_def]
+
+qspecl_then [‘b’,‘enct’] drule dec_enc_blocktype
+gvs[AllCaseEqs()]
+rewrite_tac[]
+rw[dec_enc_blocktype]
+
+    >> simp[dec_instr_def, AllCaseEqs()]
+
+simp ssa
+
+    >> simp[APPEND, dec_instr_def]
+
+
+
     >>~- ([‘dec_indxs’   ], imp_res_tac dec_enc_indxs    \\ simp[] )
     >>~- ([‘dec_functype’], imp_res_tac dec_enc_functype \\ simp[] )
     >>~- ([‘enc_varI’    ],
